test_pulse_mut.fst
@@ -1,0 +1,20 @@
+module Test
+
+#lang-pulse
+
+open Pulse.Lib.Pervasives
+module U64 = FStar.UInt64
+
+fn test_mut ()
+  requires emp
+  ensures emp
+{
+  let mut i = 1UL;
+  
+  while (U64.lte !i 10UL)
+    invariant exists* vi. pts_to i vi ** pure (U64.v vi >= 1)
+  {
+    let curr = !i;
+    i := U64.add curr 1UL
+  }
+}
