test_pulse_mut3.fst
@@ -1,0 +1,30 @@
+module Test3
+
+#lang-pulse
+
+open Pulse.Lib.Pervasives
+open Pulse.Lib.GC.Heap
+open Pulse.Lib.GC.Object
+module U64 = FStar.UInt64
+
+fn test_mut (heap: heap_t) (h_addr: hp_addr)
+  (callback: hp_addr -> stt unit (requires emp) (ensures fun _ -> emp))
+  requires is_heap heap 's
+  ensures is_heap heap 's  
+{
+  let mut i = 1UL;
+  
+  while (U64.lte !i 10UL)
+    invariant exists* vi. pts_to i vi ** is_heap heap 's ** pure (U64.v vi >= 1)
+  {
+    let curr = !i;
+    
+    let v = read_word heap h_addr;
+    
+    if (U64.gt v 0UL) {
+      callback h_addr
+    };
+    
+    i := U64.add curr 1UL
+  }
+}
